* Use the force of the length. (To be continued.)

first_structure/Buffer.v
@@ -39,15 +39,44 @@ Definition length {A : Set} (buff : t A) : nat :=
   | Five _ _ _ _ _ => 5
   end.
 
+Lemma bounded_length : forall {A} (b: t A), length b <= 5.
+Proof. 
+  destruct b; simpl; auto with arith.
+Qed.
+
+Lemma empty_length : forall {A} (b : t A), 
+  length b = 0 <-> is_empty b.
+Proof. 
+  intros A b; destruct b; simpl in * |- *; firstorder; try (congruence || auto).
+Qed.
+
+Lemma nonempty_length : forall {A} (b : t A), 
+  length b > 0 <-> ~ (is_empty b).
+Proof. 
+  intros A b; destruct b; simpl in * |- *; firstorder; try (congruence || auto).
+  inversion H.
+Qed.
+                       
 Definition color {A : Set} (buff : t A) : color :=
   match buff with
   | Zero | Five _ _ _ _ _ => Red
   | One _ | Four _ _ _ _ => Yellow
-  | _ => Red
+  | _ => Green (* Y: Il y avait Red ici, c'est bien Green non? *)
   end.
 
+Lemma length_color : 
+  forall {A} (buff : t A),
+    match color buff, length buff with
+      | Red, (0 | 5) => True
+      | Yellow, (1 | 4) => True
+      | Green, (2 | 3) => True
+      | _, _ => False
+    end.
+Proof. intros A b; destruct b; simpl; auto. Qed.
+
 Program Definition push {A : Set} (elt : A) 
-  (buff : t A | color buff <> Red \/ is_empty buff) : t A :=
+  (buff : t A | color buff <> Red \/ is_empty buff) : 
+  { buff' : t A | length buff' = S (length buff) } :=
   match buff with
   | Zero => One elt
   | One a => Two elt a
@@ -56,12 +85,12 @@ Program Definition push {A : Set} (elt : A)
   | Four a b c d => Five elt a b c d
   | Five _ _ _ _ _ => !
   end.
-
 Next Obligation.
 Proof.  firstorder. Qed.
 
 Program Definition inject {A : Set} (elt : A) 
-  (buff : t A | color buff <> Red \/ is_empty buff) : t A :=
+  (buff : t A | color buff <> Red \/ is_empty buff) : 
+  { buff' : t A | length buff' = S (length buff) } :=
   match buff with
   | Zero => One elt
   | One a => Two a elt
@@ -70,11 +99,11 @@ Program Definition inject {A : Set} (elt : A)
   | Four a b c d => Five a b c d elt
   | Five _ _ _ _ _ => !
   end.
-
 Next Obligation.
 Proof. firstorder. Qed.
 
-Program Definition pop {A : Set} (buff : t A | ~ is_empty buff) : A * t A :=
+Program Definition pop {A : Set} (buff : t A | ~ is_empty buff) : 
+  { r : A * t A | S (length (snd r)) = length buff } :=
   match buff with
   | Zero => !
   | One a => (a, Zero)
@@ -83,11 +112,11 @@ Program Definition pop {A : Set} (buff : t A | ~ is_empty buff) : A * t A :=
   | Four a b c d => (a, Three b c d)
   | Five a b c d e => (a, Four b c d e)
   end.
-
 Next Obligation.
 Proof. firstorder. Qed.
 
-Program Definition eject {A : Set} (buff : t A | ~ is_empty buff) : A * t A :=
+Program Definition eject {A : Set} (buff : t A | ~ is_empty buff) : 
+  { r : A * t A | S (length (snd r)) = length buff } :=
   match buff with
   | Zero => !
   | One a => (a, Zero)
@@ -96,6 +125,9 @@ Program Definition eject {A : Set} (buff : t A | ~ is_empty buff) : A * t A :=
   | Four a b c d => (d, Three a b c)
   | Five a b c d e => (e, Four a b c d)
   end.
-
 Next Obligation.
 Proof. firstorder. Qed.
+
+
+
+
